Spec fixes.

verified/sec_prop.i.dfy
@@ -35,6 +35,16 @@ predicate same_call_args(s1:state, s2: state)
     OperandContents(s1, OReg(R4))  == OperandContents(s2, OReg(R4))
 }
 
+predicate entering_atkr(d1: PageDb, d2: PageDb, disp: word, atkr: PageNr)
+    requires validPageDb(d1) && validPageDb(d2)
+    requires valAddrPage(d1, atkr) && valAddrPage(d2, atkr)
+{
+    validPageNr(disp) &&
+    d1[disp].PageDbEntryTyped? && d1[disp].entry.Dispatcher? &&
+    d2[disp].PageDbEntryTyped? && d2[disp].entry.Dispatcher? &&
+    d1[disp].addrspace == atkr && d2[disp].addrspace == atkr
+}
+
 lemma enc_enc_conf_ni(s1: state, d1: PageDb, s1': state, d1': PageDb,
                       s2: state, d2: PageDb, s2': state, d2': PageDb,
                       atkr: PageNr)
@@ -47,14 +57,16 @@ lemma enc_enc_conf_ni(s1: state, d1: PageDb, s1': state, d1': PageDb,
     // s.t. (s1, d1) =_{atkr} (s2, d2)
     requires enc_enc_conf_eqpdb(d1, d2, atkr)
     requires (var callno := s1.regs[R0]; var dispPage := s1.regs[R1];
-        (callno == KOM_SMC_ENTER || callno == KOM_SMC_RESUME) && dispPage == atkr 
-            ==> enc_enc_conf_eq(s1, s2, d1, d2, atkr))
+        ((callno == KOM_SMC_ENTER || callno == KOM_SMC_RESUME) && 
+            entering_atkr(d1, d2, dispPage, atkr))
+                ==> enc_enc_conf_eq(s1, s2, d1, d2, atkr))
     // then (s1', d1') =_{atkr} (s2', d2')
     ensures !(var callno := s1.regs[R0]; var asp := s1.regs[R1];
         callno == KOM_SMC_STOP && asp == atkr) ==>
         enc_enc_conf_eqpdb(d1', d2', atkr)  
     ensures (var callno := s1.regs[R0]; var dispPage := s1.regs[R1];
-        (callno == KOM_SMC_ENTER || callno == KOM_SMC_RESUME) && dispPage == atkr 
+        ((callno == KOM_SMC_ENTER || callno == KOM_SMC_RESUME) && 
+            entering_atkr(d1, d2, dispPage, atkr))
             ==> enc_enc_conf_eq(s1', s2', d1', d2', atkr))
 {
     reveal_ValidRegState();
@@ -103,9 +115,11 @@ lemma enter_enc_enc_conf_ni(s1: state, d1: PageDb, s1':state, d1': PageDb,
     requires smc_enter(s1, d1, s1', d1', dispPage, arg1, arg2, arg3)
     requires smc_enter(s2, d2, s2', d2', dispPage, arg1, arg2, arg3)
     requires enc_enc_conf_eqpdb(d1, d2, atkr)
-    requires dispPage == atkr ==> enc_enc_conf_eq(s1, s2, d1, d2, atkr)
-    ensures  enc_enc_conf_eqpdb(d1', d2', atkr)
-    ensures  dispPage == atkr ==> enc_enc_conf_eq(s1', s2', d1', d2', atkr)
+    requires entering_atkr(d1, d2, dispPage, atkr) ==>
+        enc_enc_conf_eq(s1, s2, d1, d2, atkr)
+    ensures enc_enc_conf_eqpdb(d1', d2', atkr)
+    ensures entering_atkr(d1, d2, dispPage, atkr) ==>
+        enc_enc_conf_eq(s1', s2', d1', d2', atkr)
 {
     // TODO proveme
     assume false;
@@ -119,9 +133,11 @@ lemma resume_enc_enc_conf_ni(s1: state, d1: PageDb, s1':state, d1': PageDb,
     requires smc_resume(s1, d1, s1', d1', dispPage)
     requires smc_resume(s2, d2, s2', d2', dispPage)
     requires enc_enc_conf_eqpdb(d1, d2, atkr)
-    requires dispPage == atkr ==> enc_enc_conf_eq(s1, s2, d1, d2, atkr)
-    ensures  enc_enc_conf_eqpdb(d1', d2', atkr)
-    ensures  dispPage == atkr ==> enc_enc_conf_eq(s1', s2', d1', d2', atkr)
+    requires entering_atkr(d1, d2, dispPage, atkr) ==>
+        enc_enc_conf_eq(s1, s2, d1, d2, atkr)
+    ensures enc_enc_conf_eqpdb(d1', d2', atkr)
+    ensures entering_atkr(d1, d2, dispPage, atkr) ==>
+        enc_enc_conf_eq(s1', s2', d1', d2', atkr)
 {
     // TODO proveme
     assume false;
@@ -365,22 +381,17 @@ lemma stop_enc_enc_conf_ni(d1: PageDb, d1': PageDb, e1':word,
 
 lemma enter_enc_enc_integ_ni(s1: state, d1: PageDb, s1':state, d1': PageDb,
                             s2: state, d2: PageDb, s2':state, d2': PageDb,
-                    dispPage: word, arg1: word, arg2: word, arg3: word)
-    requires SaneState(s1) && validPageDb(d1) && SaneState(s1') && validPageDb(d1')
-    requires SaneState(s2) && validPageDb(d2) && SaneState(s2') && validPageDb(d2')
-    requires pageDbCorresponds(s1.m, d1) && pageDbCorresponds(s1'.m, d1') 
-    requires pageDbCorresponds(s2.m, d2) && pageDbCorresponds(s2'.m, d2') 
-    requires validPageNr(dispPage) && valDispPage(d1, dispPage) && valDispPage(d1', dispPage)
-    // If smc_enter(s1, d1) => (s1', d1')
+                    dispPage: word, arg1: word, arg2: word, arg3: word,
+                    atkr: PageNr)
+    requires ni_reqs(s1, d1, s1', d1', s2, d2, s2', d2', atkr)
     requires smc_enter(s1, d1, s1', d1', dispPage, arg1, arg2, arg3)
-    // and smc_enter(s2, d2) => (s2', d2')
     requires smc_enter(s2, d2, s2', d2', dispPage, arg1, arg2, arg3)
-    // s.t. (s1, d1) =_{!disp} (s2, d2)
-    requires enc_enc_integ_eqpdb(d1, d2, dispPage)
-    requires enc_enc_integ_eq(s1, s2, d1, d2, dispPage)
-    // then (s1', d1') =_{!disp} (s2', d2')
-    ensures  enc_enc_integ_eqpdb(d1', d2', dispPage)
-    ensures  enc_enc_integ_eq(s1', s2', d1', d2', dispPage)
+    requires enc_enc_integ_eqpdb(d1, d2, atkr)
+    requires entering_atkr(d1, d2, dispPage, atkr) ==>
+        enc_enc_integ_eq(s1, s2, d1, d2, atkr)
+    ensures enc_enc_integ_eqpdb(d1', d2', atkr)
+    ensures entering_atkr(d1, d2, dispPage, atkr) ==>
+        enc_enc_integ_eq(s1', s2', d1', d2', atkr)
 {
     // TODO proveme
     assume false;
